src/typechecker/FStar.TypeChecker.Tc.fst
@@ -899,8 +899,13 @@ let tc_decl env se: list sigelt & list sigelt & Env.env =
     else if se.sigmeta.sigmeta_admit then (
       let result = tc_decl' { env with admit = true } se in
       result
-    ) else
-      tc_decl' env se
+    ) else (
+      FStar.SMTEncoding.Solver.set_current_decl (U.lids_of_sigelt se);
+      let result = tc_decl' env se in
+      if Options.ext_getv "profile_context" = "every_decl"
+      then FStar.SMTEncoding.Solver.report_context_current_decl ();
+      result
+    )
   in
   let () =
     (* Do the post-tc attribute/qualifier check. *)
@@ -1153,6 +1158,7 @@ let finish_partial_modul (loading_from_cache:bool) (iface_exists:bool) (en:env) 
   env.qtbl_name_and_index |> snd |> BU.smap_clear;
 
   //pop BUT ignore the old env
+
   pop_context env ("Ending modul " ^ string_of_lid m.name) |> ignore;
 
   //moved the code for encoding the module to smt to Universal
@@ -1166,7 +1172,23 @@ let tc_modul (env0:env) (m:modul) (iface_exists:bool) :(modul & env) =
   let msg = "Internals for " ^ string_of_lid m.name in
   //AR: push env, this will also push solver, and then finish_partial_modul will do the pop
   let env0 = push_context env0 msg in
+  if Options.ext_getv "profile_context" <> ""
+  then FStar.SMTEncoding.Solver.clear_profile_context();
   let modul, env = tc_partial_modul env0 m in
+  if Options.ext_getv "profile_context" <> ""
+  && not env.admit
+  then (
+    let opens = DsEnv.opens_and_abbrevs_of env.dsenv m.name in
+    let opens = opens |> List.map (function
+        | Inl (l, _, _) -> l
+        | Inr (_, l) -> l) in
+    let includes = List.collect (DsEnv.transitive_includes_of env.dsenv) opens in
+    // BU.print2 "Transitive includes of [%s] = [%s]\n"
+    //   (String.concat ", " (List.map string_of_lid opens))
+    //   (String.concat ", " (List.map string_of_lid includes));
+    let all_modules = env.modules |> List.map (fun m -> m.name) in
+    FStar.SMTEncoding.Solver.report_context_global m.name all_modules (BU.remove_dups Ident.lid_equals (opens@includes))
+  );
   // Note: all sigelts returned by tc_partial_modul must already be compressed
   // by Syntax.compress.deep_compress, so they are safe to output.
   finish_partial_modul false iface_exists env modul
